\documentclass{book}
\input{preamble.tex}
\begin{document}
\allowdisplaybreaks

\appendix

\chapter{Answers to the Exercises}\label{answers}

\renewcommand{\thechapter}{\arabic{chapter}}

\begin{answer}
If $P(E) = p$, then $P(\neg E) = 1 - p$.
\end{answer}

%% \begin{answer}%two
%%   Answer two.
%% \end{answer}

%% \begin{answer}%three
%%   Answer three.
%% \end{answer}

%% \begin{answer}%four
%%   Answer four.
%% \end{answer}

%% \begin{answer}%five
%%   Answer five.
%% \end{answer}

%% \begin{answer}%six
%%   Answer six.
%% \end{answer}

%% \begin{answer}%seven
%%   Answer seven.
%% \end{answer}

%% \begin{answer}%eight
%%   Answer eight.
%% \end{answer}

%% \begin{answer}%nine
%%   Answer nine.
%% \end{answer}

%% \begin{answer}%ten
%%   Answer ten.
%% \end{answer}

%% \begin{answer}%eleven
%%   Answer eleven.
%% \end{answer}

%% \begin{answer}%twelve
%%   Answer twelve.
%% \end{answer}


\begin{exercise*}[\ref{q:cap}]
When $E$ and $F$ are independent, finding $P(E \cap F)$ is straightforward because the sample space is simply the set of all pairs of possible outcomes from $E$ and $F$, i.e., $\Omega = \Omega_E \times \Omega_F$, where $\Omega_G$ is the sample space of an event $G$. As a result,
\begin{equation*}
P(E \cap F) = \frac{\#(E \cap F)}{|\Omega_E \times \Omega_F|}
= \frac{\#(E) \cdot \#(F)}{|\Omega_E| \cdot |\Omega_F|}
= P(E) \cdot P(F),
\end{equation*} 
where $\#(G)$ denotes the number of outcomes where event $G$ occurs (in its sample space). See Figure \ref{product} for an example.
\end{exercise*}

\begin{figure}[ht]
\centering
\input{tikz/d5timesd4.tikz}
\caption{The elements of $\Omega_{D_5} \times \Omega_{D_4}$. Let $X$ be the event where $D_5$ is prime, and let $Y$ be the event where $D_4$ is even. The outcomes where $X \cap Y$ occurs are boxed, and we can verify that $P(X \cap Y) = 6/20$ matches $P(X) \cdot P(Y) = \frac{3}{5} \cdot \frac{2}{4}$.}
\label{product}
\end{figure}


\begin{exercise*}[\ref{q:cup}]
Venn diagram properties shown in Figure \ref{vennd} reveal that for any two events $E$ and $F$, \[P(E \cup F) = P(E) + P(F) - P(E \cap F).\]
\end{exercise*}

\begin{figure}[ht]
\centering
\input{tikz/venndiagram.tikz}
\caption{A Venn diagram of two events in d6's sample space. $E$ is the event that the roll is even, and $F$ is the event that the roll is prime. So $P(E \cup F) = P(E) + P(F) - P(E \cap F) = 3/6 + 3/6 - 1/6 = 5/6$.}
\label{vennd}
\end{figure}

\begin{exercise*}[{\ref{completesquare}}] We first notice that
\[(x + h)^2 = x^2 + 2hx + h^2\] so \[\left(x + \frac{b}{2a}\right)^2 = x^2 + \frac{b}{a}x + \frac{b^2}{4a^2}.\] Then
\begin{align*}
ax^2 + bx + c &= 0\\
x^2 + \frac{b}{a}x + \frac{c}{a} &= 0\\
x^2 + \frac{b}{a}x + \frac{b^2}{4a^2} + \frac{c}{a} &= \frac{b^2}{4a^2}\\
\left(x + \frac{b}{2a}\right)^2 + \frac{c}{a} &= \frac{b^2}{4a^2}\\
\left(x + \frac{b}{2a}\right)^2 &= \frac{b^2-4ac}{4a^2}\\
x + \frac{b}{2a} &= \pm\sqrt{\frac{b^2}{4a^2}}\\
x &= \frac{-b \pm \sqrt{b^2 - 4ac}}{2a}.
\end{align*}
\end{exercise*}
\end{document}
